inv_ack_standalone.v
@@ -5,25 +5,23 @@ Require Import BinNat.
 (* ********** COUNTDOWN AND INVERSE ACKERMANN ON NAT ********** *)
 
 (* Countdown worker function *)
-Fixpoint countdown_worker (f : nat -> nat) (a n k : nat) : nat :=
+Fixpoint cdn_wkr (f : nat -> nat) (a n k : nat) : nat :=
   match k with
   | 0    => 0
   | S k' => if (n <=? a) then 0 else
-              S (countdown_worker f a (f n) k')
+              S (cdn_wkr f a (f n) k')
   end.
 
 (* Countdown *)
-Definition countdown_to f a n := countdown_worker f a n n.
+Definition countdown_to f a n := cdn_wkr f a n n.
 
 (* Inverse Ackermann worker function *)
-Fixpoint inv_ack_worker (f : nat -> nat) (n k b : nat) : nat :=
+Fixpoint inv_ack_wkr (f : nat -> nat) (n k b : nat) : nat :=
   match b with
-  | 0    => k
-  | S b' => match (n - k) with
-            | 0   => k
-            | _ => let g := (countdown_to f 1) in
-                     inv_ack_worker (compose g f) (g n) (S k) b'
-            end
+  | 0      => k
+  | S b' => if (n <=? k) then k
+              else let g := (countdown_to f 1) in
+                   inv_ack_wkr (compose g f) (g n) (S k) b'
   end.
 
 (* Inverse Ackermann function *)
@@ -31,8 +29,23 @@ Fixpoint inv_ack_worker (f : nat -> nat) (n k b : nat) : nat :=
 Definition inv_ack_linear n :=
   match n with
   | 0 | 1 => 0
-  | _     => let f := (fun x => x - 2) in inv_ack_worker f (f n) 1 (n - 1)
+  | _     => let f := (fun x => x - 2) in inv_ack_wkr f (f n) 1 (n - 1)
   end.
+
+(* Two parameters Inverse Ackerman worker function *)
+Fixpoint two_params_inv_ack_wkr (f : nat -> nat) (n k b : nat) : nat :=
+  match b with
+  | 0    => k
+  | S b' => if (n <=? k) then 0
+              else let g := (countdown_to f 1) in
+                   S (two_params_inv_ack_wkr (compose g f) (g n) k b')
+  end.
+
+(* Two parameters Inverse Ackermann function *)
+Definition two_params_inv_ack (m n : nat) : nat :=
+  let f := (fun x => x - 2) in
+    let n' := (Nat.log2_up n) in
+      1 + two_params_inv_ack_wkr f (f n') (Nat.div m n) n'.
 
 
 (* ********** COUNTDOWN AND INVERSE ACKERMANN ON N (BINARY) ********** *)
@@ -64,13 +77,13 @@ Definition bin_countdown_to (f : N -> N) (a n : N) : N
   := bin_cdn_wkr f a n (nat_size (n - a)).
 
 (* Inverse Ackermann worker function *)
-Fixpoint bin_inv_ack_worker (f : N -> N) (n k : N) (bud : nat) : N :=
-  match bud with
+Fixpoint bin_inv_ack_wkr (f : N -> N) (n k : N) (b : nat) : N :=
+  match b with
   | 0%nat  => k
-  | S bud' =>
+  | S b' =>
     if n <=? k then k
       else let g := (bin_countdown_to f 1) in
-      bin_inv_ack_worker (compose g f) (g n) (N.succ k) bud'
+      bin_inv_ack_wkr (compose g f) (g n) (N.succ k) b'
   end.
 
 (* Inverse Ackermann function *)
@@ -80,4 +93,19 @@ Definition bin_inv_ack n :=
   else if (n <=? 3) then 1
   else if (n <=? 7) then 2
   else let f := (fun x => N.log2 (x + 2) - 2) in
-        bin_inv_ack_worker f (f n) 3 (nat_size n).
+        bin_inv_ack_wkr f (f n) 3 (nat_size n).
+
+(* Two parameters Inverse Ackerman worker function *)
+Fixpoint two_params_bin_inv_ack_wkr (f : N -> N) (n k : N) (b : nat) : N :=
+  match b with
+  | 0%nat => k
+  | S b'  => if (n <=? k) then 0
+              else let g := (bin_countdown_to f 1) in
+                   N.succ (two_params_bin_inv_ack_wkr (compose g f) (g n) k b')
+  end.
+
+(* Two parameters Inverse Ackermann function *)
+Definition two_params_bin_inv_ack (m n : N) : N :=
+  let f := (fun x => x - 2) in
+    let n' := (N.log2_up n) in
+      1 + two_params_bin_inv_ack_wkr f (f n') (N.div m n) (nat_size n).
